Fix pan_to_crepProof for exception declarations

pancake/pan_to_crepScript.sml
@@ -368,13 +368,7 @@ End
 (* extract eids from exception declarations *)
 Definition get_eids_from_decls_def:
   get_eids_from_decls (decls:'a decl list) =
-    let eids =
-          FOLDR
-            (λd acc.
-               case d of
-               | ExnDecl eid sh => eid :: acc
-               | _              => acc)
-            [] decls;
+    let eids = MAP FST (exceptions decls);
         (*eids = nub eids;*)
         ns   = GENLIST (λx. (n2w x):'a word) (LENGTH eids);
         es   = MAP2 (λx y. (x,y)) eids ns
